adapted the stateful-encryption framed example; still getting transient errors

examples/security/statefulEnc-multi-frame.fst
@@ -2,7 +2,7 @@
     options:--admit_fsi Set --admit_fsi Seq --z3timeout 15 --max_fuel 1 --max_ifuel 1 --initial_ifuel 1 --max_ifuel 1;
     other-files:../../lib/ext.fst ../../lib/set.fsi ../../lib/heap.fst ../../lib/st.fst ../../lib/seq.fsi ../../lib/list.fst
   --*)
-(* A standalone experiment corresponding to building a stateful encryption on
+(* A standalone experiment corresponding to building stateful encryption on
    top of a stateless one ... along the lines of StatefulLHAE on top of AEAD_GCM *)
 module StatefulEncryption.MultiInstance.Frame
 open ST
@@ -37,6 +37,9 @@ let rec find_seq' a f s i =
 let find_seq a f s = find_seq' #a f s 0
 *)
 
+assume val seq_map: #a:Type -> #b:Type -> f:(a -> Tot b) -> s:seq a ->
+  Tot (t:seq b { Seq.length t = Seq.length s /\ (forall (i:nat{i < Seq.length s}).(Seq.index t i = f (Seq.index s i))) })
+
 // replacing the usual modifies clause?
 // this does not preclude h' extending h with fresh refs
 opaque logic type modifies (mods:set aref) (h:heap) (h':heap) =
@@ -47,29 +50,34 @@ type Fresh (#a:Type) h0 (r:ref a) h1 = Heap.contains h1 r /\ not (Heap.contains 
 type Let (#a:Type) (x:a) (body: (y:a{y=x} -> Type)) = body x
 
 (* ------------------------------------------------------------ *)
-(* Start with a basic stateful encryption functionality *)
+(* Start with a basic possibly-stateful encryption functionality *)
 
 (* Some placeholder functions to build plain/cipher/key *)
 
 type key
-// we need something more stateful, accounting for random sampling & pairwise distinct keys
+// we need something possibly stateful, accounting for random sampling & pairwise distinct keys
 // similarly we should be able to instantiate the scheme to an instance that holds/updates refs in key
 
-// assume val mk_key: unit -> Tot key
-assume val mk_key: unit -> St key (fun h -> True) (fun h0 k h1 -> modifies !{} h0 h1)
+// assume val gen0: unit -> Tot key
+assume val gen0: unit -> St key (fun h -> True) (fun h0 k h1 -> modifies !{} h0 h1)
 
 type plain
 assume val mk_plain: unit -> St plain (fun h -> True) (fun h0 k h1 -> modifies !{} h0 h1)
 
+type ad = nat // additional data, just integers for simplicity
+
 type cipher
-assume val mk_cipher: unit -> St cipher (fun h -> True) (fun h0 k h1 -> modifies !{} h0 h1)
+assume val enc0: s:seq cipher (* ghost *) -> St cipher
+  (fun h -> True)
+  (fun h0 c h1 -> modifies !{} h0 h1
+               /\ find_seq (fun c' -> c=c') s = None)
 
 // to guarantees that decryption is a stateful inverse of encryption (a good sanity check),
 // the invariant on entries should state that the ciphers are pairwise distinct.
 // we may also have a refinement guaranteeing that decryption of that ciphertext yields that plaintext.
 
 type basicEntry =
-  | Entry : p:plain -> c:cipher -> basicEntry
+  | Entry : i:ad -> c:cipher -> p:plain -> basicEntry
 
 type encryptor =
   | Enc : log:ref (seq basicEntry) -> key -> encryptor
@@ -118,7 +126,7 @@ val gen: unit -> St bi
          Fresh h0 log h1
          /\ Heap.sel h1 log = emp)))
 let gen () =
-  let key = mk_key () in
+  let key = gen0 () in
   let log = ref emp in
   let bi = BI (Enc log key) (Dec log key) in
   basic_fp := bi::!basic_fp; //ghost
@@ -131,36 +139,38 @@ type in_basic_fp bi h =
 type enc_in_basic_fp (e:encryptor) (h:heap) = exists d. paired e d /\ in_basic_fp (BI e d) h
 type dec_in_basic_fp (d:decryptor) (h:heap) = exists e. paired e d /\ in_basic_fp (BI e d) h
 
-val enc : e:encryptor -> p:plain -> St cipher
+val enc : e:encryptor -> i:ad -> p:plain -> St cipher
     (requires (fun h -> enc_in_basic_fp e h))
     (ensures (fun h0 c h1 ->
                 modifies !{Enc.log e} h0 h1
                 /\ enc_in_basic_fp e h1
                 // /\ Heap.contains h1 (Enc.log e) // could we get it from the precondition?
-                /\ Heap.sel h1 (Enc.log e) = snoc (Heap.sel h0 (Enc.log e)) (Entry p c)))
-let enc e p =
-  let c = mk_cipher () in
-  Enc.log e := snoc !(Enc.log e) (Entry p c);
+                /\ Heap.sel h1 (Enc.log e) = snoc (Heap.sel h0 (Enc.log e)) (Entry i c p)))
+let enc e i p =
+  // failing: let s = seq_map #basicEntry #cipher (fun (e:basicEntry) -> Entry.c e) !(Enc.log e) in
+  let c = enc0 emp in
+  Enc.log e := snoc !(Enc.log e) (Entry i c p);
   c
 
+let basicMatch i c (Entry i' c' p) = i = i' && c = c'
+
 // cryptographically, this assumes both INT-CTXT and IND-CPA (except for distinct ciphers)
-val dec: d:decryptor -> c:cipher -> St (option plain)
+val dec: d:decryptor -> a:ad -> c:cipher -> St (option plain)
   (requires (fun h -> dec_in_basic_fp d h))
-  (ensures (fun h0 p h1 ->
+  (ensures (fun h0 o h1 ->
               modifies !{} h0 h1
               /\ dec_in_basic_fp d h1
               /\ (Let (Heap.sel h0 (Dec.log d))
                       (fun log ->
-                          (is_None p <==> (forall (i:nat{i < Seq.length log}).{:pattern (trigger i)} trigger i /\ Entry.c (Seq.index log i) <> c))
-                          /\ (is_Some p ==> (exists (i:nat{i < Seq.length log}).{:pattern (trigger i)} trigger i /\ Seq.index log i = Entry (Some.v p) c))))))
-let dec d c =
+                          (is_None o <==> (forall (i:nat{i < Seq.length log}).{:pattern (trigger i)} trigger i /\ ~(basicMatch a c (Seq.index log i))))
+                          /\ (is_Some o ==> (exists (i:nat{i < Seq.length log}).{:pattern (trigger i)} trigger i /\ basicMatch a c (Seq.index log i) /\ Entry.p (Seq.index log i) = Some.v o))))))
+let dec d a c =
   let s = !(Dec.log d) in
-  match find_seq (function Entry p c' -> c=c') s with
+  match find_seq (basicMatch a c) s with
     | None -> None
     | Some i ->
       cut (trigger i);
       Some (Entry.p (Seq.index s i))
-
 
 val test_basic_frame : b1:bi -> b2:bi{distinct_bi b1 b2} -> St unit
     (requires (fun h ->
@@ -178,21 +188,23 @@ let test_basic_frame b1 b2 =
   // let b3 = gen() in // this breaks typing; why?
   let p = mk_plain () in
   let q = mk_plain () in
-  let c1 = enc (BI.e b1) p in
-  //  let c1'= enc (BI.e b1) q in // this breaks typing, unless we strengthen our invariant
-  let c2 = enc (BI.e b2) q in
-  let p' = dec (BI.d b1) c1 in
-  let q' = dec (BI.d b2) c2 in
-  cut (trigger 0);
-  assert (Some.v p' = p);
-  assert (Some.v q' = q)
+  let c0 = enc (BI.e b1) 0 p in
+  let c1 = enc (BI.e b1) 1 q in
+  let c2 = enc (BI.e b2) 0 q in
+  let o0 = dec (BI.d b1) 0 c0 in
+  let o2 = dec (BI.d b2) 0 c2 in
+  let oX = dec (BI.d b1) 2 c0 in // this fails with 1, as we might have c0=c1
+  cut (trigger 0); // what does this achieve?
+  assert (Some.v o0 = p);
+  assert (Some.v o2 = q);
+  assert (oX = None)
 
 (* -------------------------------------------------------- *)
 (* This is the analog of StatefulLHAE on top of AEAD_GCM *)
 type statefulEntry =
-  | StEntry : i:nat -> p:plain -> c:cipher -> statefulEntry
+  | StEntry : c:cipher -> p:plain -> statefulEntry
 
-// it is a bit strange to have a copy of the sequence index
+// we used to have a copy of i inside each entry; now gone
 // as above, we could use a stronger invariant
 
 type st_encryptor =
@@ -215,10 +227,7 @@ type st_paired (enc:st_encryptor) (dec:st_decryptor) =
 type sti =
   | STI : e:st_encryptor -> d:st_decryptor{st_paired e d} -> sti
 
-(* an abstract function to add additional data to the plain text *)
-assume val with_seqn : nat -> plain -> Tot plain
 // this is simplified from AEAD (usually not encrypted)
-// we will need it to be injective in its first argument
 
 (* The invariant of a single instance *)
 type st_inv (e:st_encryptor) (d:st_decryptor) (h:heap) =
@@ -236,8 +245,7 @@ type st_inv (e:st_encryptor) (d:st_decryptor) (h:heap) =
       /\ r <= w              //read counter is before it
       /\ (forall (i:nat{i < Seq.length st}).
           Let (Seq.index st i) (fun st_en ->
-            StEntry.i st_en = i  //the log is in sync with the basic log, with the ith entry containing i as the additional data
-            /\ Seq.index basic i = Entry (with_seqn i (StEntry.p st_en)) (StEntry.c st_en)))))))
+            b2t (Seq.index basic i = Entry i (StEntry.c st_en) (StEntry.p st_en) )))))))
 
 type st_enc_inv (e:st_encryptor) (h:heap) =
   exists (d:st_decryptor). st_paired e d /\ st_inv e d h
@@ -289,80 +297,75 @@ let stateful_gen () =
   st_fp := sti :: !st_fp; //ghost
   sti
 
-let in_st_fp sti h = List.mem sti (Heap.sel h st_fp)
+type in_st_fp sti h =
+  st_fp_inv h /\
+  b2t( List.mem sti (Heap.sel h st_fp))
 
-type enc_in_st_fp (e:st_encryptor) (h:heap) =
-  exists d. st_paired e d /\ in_st_fp (STI e d) h
-
-type dec_in_st_fp (d:st_decryptor) (h:heap) =
-  exists e. st_paired e d /\ List.mem (STI e d) (Heap.sel h st_fp)
+type enc_in_st_fp (e:st_encryptor) (h:heap) = exists d. st_paired e d /\ in_st_fp (STI e d) h
+type dec_in_st_fp (d:st_decryptor) (h:heap) = exists e. st_paired e d /\ in_st_fp (STI e d) h
 
 val stateful_enc : e:st_encryptor -> p:plain -> St cipher
-  (requires (fun h -> st_fp_inv h /\ enc_in_st_fp e h))
+  (requires (fun h -> enc_in_st_fp e h))
   (ensures (fun h0 c h1 ->
-                 st_fp_inv h1
+                    enc_in_st_fp e h1
                  /\ modifies (refs_in_e e) h0 h1
                  /\ Heap.sel h1 (StEnc.log e) //exactly plain added to the end of the log
-                    = snoc (Heap.sel h0 (StEnc.log e)) (StEntry (Heap.sel h0 (StEnc.ctr e)) p c)))
-let stateful_enc e p =
-  //let h0 = get() in
-  let i = !(StEnc.ctr e) in
-  let ip = with_seqn i p in
-  let c = enc (StEnc.key e) ip in
-  StEnc.log e := snoc !(StEnc.log e) (StEntry i p c);
-  StEnc.ctr e := i + 1;
+                     = snoc (Heap.sel h0 (StEnc.log e)) (StEntry c p)))
+let stateful_enc (StEnc log ctr e) p =
+  let c = enc e !ctr p in
+  log := snoc !log (StEntry c p);
+  ctr := !ctr + 1;
   c
 
-
-val stateful_dec: ad:nat -> d:st_decryptor -> c:cipher -> St (option plain)
-  (requires (fun h -> st_fp_inv h /\ dec_in_st_fp d h))
+val stateful_dec: d:st_decryptor -> c:cipher -> St (option plain)
+  (requires (fun h -> dec_in_st_fp d h))
   (ensures (fun h0 p h1 ->
-                st_fp_inv h0
-                /\ dec_in_st_fp d h0 //repeating pre
-                /\ st_fp_inv h1
+                   dec_in_st_fp d h0 //repeating pre
+                /\ dec_in_st_fp d h1
                 /\ modifies !{StDec.ctr d} h0 h1
                 /\ Let (Heap.sel h0 (StDec.ctr d)) (fun (r:nat{r=Heap.sel h0 (StDec.ctr d)}) ->
                    Let (Heap.sel h0 (StDec.log d)) (fun (log:seq statefulEntry{log=Heap.sel h0 (StDec.log d)}) ->
                     (is_None p ==> (r = Seq.length log                     //nothing encrypted yet
-                                    || StEntry.c (Seq.index log r) <> c    //bogus cipher
-                                    || r <> ad))                           //reading at the wrong postition
+                                    || StEntry.c (Seq.index log r) <> c    //wrong cipher
+                                    ) /\ Heap.sel h1 (StDec.ctr d) = r)
                    /\ (is_Some p ==>
                           ((Heap.sel h1 (StDec.ctr d) = r + 1)
                            /\ StEntry.p (Seq.index log r) = Some.v p))))))
-let stateful_dec ad d c =
-  let i = !(StDec.ctr d) in
-  cut(trigger i);
-  match dec (StDec.key d) c with
-    | None ->  None
-    | Some p ->
-      let l = !(StDec.log d) in
-      if i < Seq.length l
-      then let StEntry _ q _ = Seq.index l i in
-           if i = ad
-           then (StDec.ctr d := i + 1; Some q)
-           else None
-      else None
 
+// note that we do not increment the counter in case of decryption failure,
+// thereby enabling retries
+let stateful_dec (StDec _ ctr d) c =
+  let i = !ctr in
+  cut(trigger i); // what does it do?
+  match dec d !ctr c with
+    | None -> None
+    | Some p -> ctr := !ctr + 1; Some p
+
+// what does it do? related to transient failures?
 #reset-options
 val test_st_frame : s1:sti -> s2:sti{distinct_sti s1 s2} -> St unit
-    (requires (fun h -> st_fp_inv h
-                    /\ in_st_fp s1 h
-                    /\ in_st_fp s2 h
-                    /\ Heap.sel h (StEnc.ctr (STI.e s1))
-                       = Heap.sel h (StDec.ctr (STI.d s1))
-                    /\ Heap.sel h (StEnc.ctr (STI.e s2))
-                       = Heap.sel h (StDec.ctr (STI.d s2))))
+    (requires (fun h ->
+                   in_st_fp s1 h
+                /\ in_st_fp s2 h
+                /\ Heap.sel h (StEnc.ctr (STI.e s1)) = Heap.sel h (StDec.ctr (STI.d s1))
+             // /\ Heap.sel h (StEnc.ctr (STI.e s2)) = Heap.sel h (StDec.ctr (STI.d s2))
+                    ))
     (ensures (fun h0 _ h1 ->
-                st_fp_inv h1
+                   in_st_fp s1 h1
+                /\ in_st_fp s2 h1
                 /\ modifies (Set.union (sti_refs s1) (sti_refs s2)) h0 h1))
+// note that we do not require new encryptor/decryptors,
+// just that those in s1 are in sync, so that decryption cancels encryption
+
 let test_st_frame s1 s2 =
-  let p1 = mk_plain () in
-  let p2 = mk_plain () in
-  let c1 = stateful_enc (STI.e s1) p1 in
-  let c2 = stateful_enc (STI.e s2) p2 in
-  let n1 = !(StDec.ctr (STI.d s1)) in
-  let p1' = stateful_dec n1 (STI.d s1) c1 in
-  let n2 = !(StDec.ctr (STI.d s2)) in
-  let p2' = stateful_dec n2 (STI.d s2) c2 in
-  assert (is_Some p1' /\ Some.v p1' = p1);
-  assert (is_Some p2' /\ Some.v p2' = p2)
+  let p = mk_plain () in
+  let q = mk_plain () in
+  // let s3 = stateful_gen() // also type-breaking
+  let c0 = stateful_enc (STI.e s1) p in
+  let c1 = stateful_enc (STI.e s1) q in
+  let c2 = stateful_enc (STI.e s2) p in
+  // let oX = stateful_dec (STI.d s1) c2 in // might succeed
+  let o0 = stateful_dec (STI.d s1) c0 in
+  let o1 = stateful_dec (STI.d s1) c1 in
+  assert (Some.v o0 = p);
+  assert (Some.v o1 = q)
